

$$f(t) = \begin{cases} t, & 0 \leq t \leq 1 \\ 2-t, & 1 \leq t \leq 2 \\ 0, & t > 2 \end{cases}$$

$$f(t) = t[u(t) - u(t-1)] + (2-t)[u(t-1) - u(t-2)]$$

$$t u(t-a) = (t-a) u(t-a) + a u(t-a)$$

$$f(t) = t u(t) - t u(t-1) + 2 u(t-1) - t u(t-1) - 2 u(t-2) + t u(t-2)$$

$$= t u(t) - [(t-1) u(t-1) + u(t-1)] + 2 u(t-1) - [(t-1) u(t-1) + u(t-1)] - 2 u(t-2) + [(t-2) u(t-2) + 2 u(t-2)]$$

$$f(t) = t u(t) - 2(t-1) u(t-1) + (t-2) u(t-2) = r(t) - 2r(t-1) + r(t-2)$$



$$r(t) = tu(t), \mathcal{L}\{r(t)\} = \frac{1}{s^2}, \mathcal{L}\{r(t-a)\} = e^{-as} \frac{1}{s^2}$$

$$f(s) = \mathcal{L}\{f(t)\} = \frac{1}{s^2} - \frac{2e^{-s}}{s^2} + \frac{e^{-2s}}{s^2} = \frac{(1-e^{-s})^2}{s^2}$$